ovn/proofs/ssprove/extraction/ConCertLib.v
@@ -1,0 +1,140 @@
+Set Warnings "-notation-overridden,-ambiguous-paths".
+From Crypt Require Import choice_type Package Prelude.
+Import PackageNotation.
+From extructures Require Import ord fset.
+From mathcomp Require Import ssrZ word.
+From Jasmin Require Import word.
+
+From Coq Require Import ZArith.
+From Coq Require Import Strings.String.
+   Import List.ListNotations.
+Open Scope list_scope.
+Open Scope Z_scope.
+Open Scope bool_scope.
+
+From Hacspec Require Import ChoiceEquality.
+From Hacspec Require Import LocationUtility.
+From Hacspec Require Import Hacspec_Lib_Comparable.
+From Hacspec Require Import Hacspec_Lib_Pre.
+From Hacspec Require Import Hacspec_Lib.
+
+Open Scope hacspec_scope.
+Import choice.Choice.Exports.
+
+From Hacspec Require Import ChoiceEquality.
+From Hacspec Require Import LocationUtility.
+From Hacspec Require Import Hacspec_Lib_Comparable.
+From Hacspec Require Import Hacspec_Lib_Pre.
+From Hacspec Require Import Hacspec_Lib.
+
+From Coq Require Import Morphisms ZArith.
+From Coq Require Import List.
+Import ListNotations.
+Open Scope Z_scope.
+Open Scope bool_scope.
+Open Scope hacspec_scope.
+
+(* From QuickChick Require Import QuickChick. *)
+(* Require Import QuickChickLib. *)
+
+From ConCert.Execution Require Import Serializable.
+From ConCert.Execution Require Import Blockchain.
+
+(* Require Import Hacspec_Concordium. *)
+(* Export Hacspec_Concordium. *)
+
+Global Program Instance int_serializable {ws : wsize} : Serializable (int ws) :=
+  {| serialize m := (serialize (unsigned m)) ;
+    deserialize l := option_map (fun (x : Z) => @repr ws x) (deserialize l) |}.
+Next Obligation.
+  intros. hnf. rewrite deserialize_serialize.
+  unfold option_map. now rewrite wrepr_unsigned.
+Defined.
+
+(* Global Program Instance nseq_serializable len : Serializable (nseq int8 len) := *)
+(*   {| serialize m := (serialize (nat_from_be_bytes m)) ; *)
+(*     deserialize l := option_map (fun (x : nat) => nat_to_be_bytes x) (deserialize l) |}. *)
+(* Next Obligation. *)
+(*   intros. cbn. rewrite deserialize_serialize. cbn. rewrite nat_to_from_be_bytes. reflexivity. *)
+(* Defined. *)
+
+(* Global Program Instance nseq_countable len : countable.Countable (nseq int8 len) := *)
+(* {| *)
+(*     countable.encode := fun X : nseq int8 _ => countable.encode (nat_from_be_bytes X); *)
+(*     countable.decode := fun H : positive => option_map (@nat_to_be_bytes _) (countable.decode H : option nat); *)
+(* |}. *)
+(* Next Obligation. *)
+(*   intros. *)
+(*   rewrite countable.decode_encode. *)
+(*   cbn. *)
+(*   now rewrite nat_to_from_be_bytes. *)
+(* Qed. *)
+
+Instance BaseTypes : ChainBase := {|
+    Address := int32;
+    address_eqb := Hacspec_Lib_Comparable.eqb ;
+    address_eqb_spec := Hacspec_Lib_Comparable.eqbP ;
+    (* address_eqdec x y := (EqDecIsDecidable x y); *)
+    address_countable := (* nseq_countable *) _;
+    address_serializable := (* nseq_serializable *) _;
+    address_is_contract := (fun x => Nat.even ((* nat_from_be_bytes x *) Z.to_nat (unsigned x))); |}.
+
+(* Definition context_t_from_context (ctx : ContractCallContext) : context_t := *)
+(*   (ctx.(ctx_from), ctx.(ctx_origin), repr (ctx.(ctx_amount))). *)
+
+(* Definition accept (ctx : ContractCallContext) := act_transfer ctx.(ctx_origin) ctx.(ctx_amount). *)
+
+(* Definition has_action_t := ActionBody. *)
+
+(* Definition action_body_t := ActionBody. *)
+(* Definition list_action_t := list ActionBody. *)
+(* Definition ACT_TRANSFER (p : Address ∏ int64) := act_transfer (fst p) (unsigned (snd p)).   *)
+(* Instance d_ab : Default ActionBody := {| default := act_transfer (array_new_ (default : int8) 32) 0 |}. *)
+
+(* Program Definition to_action_body (ctx : ContractCallContext) (y : has_action_t) : ActionBody := *)
+(*   match y with *)
+(*   | (Accept _) => act_transfer (ctx.(ctx_from)) (ctx.(ctx_amount)) *)
+(*   | (SimpleTransfer (ua, i)) => act_transfer (ua) (i) *)
+(*   | (SendRaw (ua, receive_name, amount, data)) => *)
+(*       act_call (ua) (amount) (list_rect (fun _ : list int8 => SerializedValue) *)
+(*                                         (build_ser_value ser_unit tt) *)
+(*                                         (fun a _ IHdata => *)
+(*                                            build_ser_value *)
+(*                                              (ser_pair ser_int (ser_value_type IHdata)) *)
+(*                                              (unsigned a, ser_value IHdata)) *)
+(*                                         data) *)
+(*   end. *)
+(* Instance default_has_action : Default has_action_t := {| default := Accept tt |}. *)
+
+(* Global Instance serializable_has_action_t : Serializable has_action_t := *)
+(*   Derive Serializable has_action_t_rect<Accept,SimpleTransfer,SendRaw>. *)
+(* Global Instance show_has_action_t : Show (has_action_t) := *)
+(*  @Build_Show (has_action_t) (fun x => *)
+(*  match x with *)
+(*  Accept a => ("Accept" ++ show a)%string *)
+(*  | SimpleTransfer a => ("SimpleTransfer" ++ show a)%string *)
+(*  | SendRaw a => ("SendRaw" ++ show a)%string *)
+(*  end). *)
+(* Definition g_has_action_t : G (has_action_t) := oneOf_ (bindGen arbitrary (fun a => returnGen (Accept a))) [bindGen arbitrary (fun a => returnGen (Accept a));bindGen arbitrary (fun a => returnGen (SimpleTransfer a))]. *)
+(* Global Instance gen_has_action_t : Gen (has_action_t) := Build_Gen has_action_t g_has_action_t. *)
+
+(* Definition to_action_body_list (ctx : ContractCallContext) {X} (k : option (X ∏ list has_action_t)) : ResultMonad.result (X ∏ list ActionBody) unit  := *)
+(*   match (option_map (fun '(x, y) => (x, List.map (to_action_body ctx) y)) k) with *)
+(*     Some a => ResultMonad.Ok a *)
+(*   | None => ResultMonad.Err tt *)
+(*   end. *)
+
+
+(* Instance show_user_address_t : Show (user_address_t) := Build_Show (user_address_t) show. *)
+(* Definition g_user_address_t : G (user_address_t) := arbitrary. *)
+(* Instance gen_user_address_t : Gen (user_address_t) := Build_Gen user_address_t g_user_address_t. *)
+
+(* Global Instance serializable_context_t : Serializable context_t := *)
+(*   Derive Serializable context_t_rect<Context>. *)
+(* Global Instance show_context_t : Show (context_t) := *)
+(*  @Build_Show (context_t) (fun x => *)
+(*  match x with *)
+(*  Context a => ("Context" ++ show a)%string *)
+(*  end). *)
+(* Definition g_context_t : G (context_t) := oneOf_ (bindGen arbitrary (fun a => returnGen (Context a))) [bindGen arbitrary (fun a => returnGen (Context a))]. *)
+(* Global Instance gen_context_t : Gen (context_t) := Build_Gen context_t g_context_t. *)
